yalla/ill_cut_at.v
@@ -20,127 +20,99 @@ Variable P_gax_cut : forall b l1 l2, fst (projT2 (ipgax P) b) = l1 ++ ivar X :: 
 Lemma subs_gax_l l0 l1 l2 b : fst (projT2 (ipgax P) b) = l1 ++ ivar X :: l2 ->
   ill P l0 (ivar X) -> ill P (l1 ++ l0 ++ l2) (snd (projT2 (ipgax P) b)).
 Proof using P_gax_noN_l P_gax_cut.
-intros Hb pi.
-remember (ivar X) as A eqn:HeqX.
+intros Hb pi. remember (ivar X) as A eqn:HeqX.
 induction pi; inversion HeqX; subst;
   try (list_simpl; rewrite app_assoc; constructor;
        list_simpl; rewrite ? app_comm_cons, (app_assoc l0); apply IHpi; assumption).
-- cbn; rewrite <- Hb; apply (gax_ir b).
+- cbn. rewrite <- Hb. apply (gax_ir b).
 - apply (ex_ir (l1 ++ l0 ++ l2)).
   + apply IHpi; assumption.
-  + apply PEPermutation_Type_app_head, PEPermutation_Type_app_tail; assumption.
-- list_simpl; rewrite app_assoc.
-  eapply ex_oc_ir; [ | eassumption ].
-  list_simpl; rewrite (app_assoc l0), (app_assoc _ l3), <- (app_assoc l0).
-  apply IHpi; assumption.
-- list_simpl; rewrite app_assoc.
-  apply lpam_ilr; [ assumption | ].
-  list_simpl; rewrite ? app_comm_cons, (app_assoc l3).
-  apply IHpi2; assumption.
-- exfalso.
-  apply (P_gax_noN_l b).
-  rewrite Hb.
-  apply in_inf_elt.
-- list_simpl; rewrite app_assoc.
-  apply lmap_ilr; [ assumption | ].
-  list_simpl; rewrite app_comm_cons, (app_assoc l3).
-  apply IHpi2; assumption.
-- exfalso.
-  apply (P_gax_noN_l b).
-  rewrite Hb.
-  apply in_inf_elt.
-- list_simpl; rewrite app_assoc.
-  apply plus_ilr; list_simpl; rewrite app_comm_cons, (app_assoc l0);
-    [ apply IHpi1 | apply IHpi2 ]; assumption.
-- list_simpl; rewrite app_assoc.
-  apply cut_ir with A; try assumption.
-  list_simpl; rewrite app_comm_cons, (app_assoc l3).
-  apply IHpi2; assumption.
-- destruct (P_gax_cut b _ _ Hb a eq_refl) as [? -> ->].
-  apply gax_ir.
+  + apply PEPermutation_Type_app_head, PEPermutation_Type_app_tail. assumption.
+- list_simpl. rewrite app_assoc. eapply ex_oc_ir; [ | eassumption ].
+  list_simpl. rewrite (app_assoc l0), (app_assoc _ l3), <- (app_assoc l0). apply IHpi; assumption.
+- list_simpl. rewrite app_assoc. apply lpam_ilr; [ assumption | ].
+  list_simpl. rewrite ? app_comm_cons, (app_assoc l3). apply IHpi2; assumption.
+- exfalso. apply (P_gax_noN_l b). rewrite Hb. apply in_inf_elt.
+- list_simpl. rewrite app_assoc. apply lmap_ilr; [ assumption | ].
+  list_simpl. rewrite app_comm_cons, (app_assoc l3). apply IHpi2; assumption.
+- exfalso. apply (P_gax_noN_l b). rewrite Hb. apply in_inf_elt.
+- list_simpl. rewrite app_assoc.
+  apply plus_ilr; list_simpl; rewrite app_comm_cons, (app_assoc l0); [ apply IHpi1 | apply IHpi2 ]; assumption.
+- list_simpl. rewrite app_assoc. apply cut_ir with A; [ assumption .. | ].
+  list_simpl. rewrite app_comm_cons, (app_assoc l3). apply IHpi2; assumption.
+- destruct (P_gax_cut b _ _ Hb a eq_refl) as [? -> ->]. apply gax_ir.
 Qed.
 
 Lemma cut_at_ir_gax l0 l1 l2 C :
   ill P l0 (ivar X) -> ill P (l1 ++ ivar X :: l2) C -> ill P (l1 ++ l0 ++ l2) C.
 Proof using P_gax_noN_l P_gax_cut.
-intros pi1 pi2.
-remember (l1 ++ ivar X :: l2) as l eqn:Heql; induction pi2 in l1, l2, Heql |- *; subst;
+intros pi1 pi2. remember (l1 ++ ivar X :: l2) as l eqn:Heql.
+induction pi2 in l1, l2, Heql |- *; subst;
   try (constructor; list_simpl; rewrite ? app_comm_cons; apply IHpi2; list_simpl; reflexivity);
   try (trichot_elt_elt_inf_exec Heql;
-       [ list_simpl; constructor;
-         rewrite ? app_comm_cons, app_assoc; apply IHpi2; list_simpl; reflexivity
+       [ list_simpl; constructor; rewrite ? app_comm_cons, app_assoc; apply IHpi2; list_simpl; reflexivity
        | inversion Heql1
        | rewrite 2 app_assoc; constructor; list_simpl; apply IHpi2; list_simpl; reflexivity ]).
-- unit_vs_elt_inv Heql; inversion Heql; subst; list_simpl; assumption.
+- unit_vs_elt_inv Heql. injection Heql as [= ->]. list_simpl. assumption.
 - apply PEPermutation_Type_vs_elt_subst in p as [(l4, l5) HP ->].
-  specialize (HP l0); symmetry in HP.
-  refine (ex_ir _ _ _ _ HP).
-  apply IHpi2; reflexivity.
+  specialize (HP l0). symmetry in HP. refine (ex_ir _ _ _ _ HP).
+  apply IHpi2. reflexivity.
 - dichot_elt_app_inf_exec Heql; subst.
-  + rewrite 2 app_assoc.
-    eapply ex_oc_ir; [ | eassumption ].
-    list_simpl; apply IHpi2; list_simpl; reflexivity.
+  + rewrite 2 app_assoc. eapply ex_oc_ir; [ | eassumption ].
+    list_simpl. apply IHpi2. list_simpl. reflexivity.
   + dichot_elt_app_inf_exec Heql1; subst.
-    * symmetry in Heql0; decomp_map_inf Heql0; inversion Heql0.
-    * rewrite <- 2 app_assoc.
-      eapply ex_oc_ir; [ | eassumption ].
-      rewrite 2 app_assoc; apply IHpi2; list_simpl; reflexivity.
-- destruct l1; inversion Heql.
+    * symmetry in Heql0. decomp_map_inf Heql0. discriminate Heql0.
+    * rewrite <- 2 app_assoc. eapply ex_oc_ir; [ | eassumption ]. rewrite 2 app_assoc.
+      apply IHpi2. list_simpl. reflexivity.
+- nil_vs_elt_inv Heql.
 - dichot_elt_app_inf_exec Heql; subst.
-  + rewrite 2 app_assoc; apply tens_irr; [ | assumption ].
-    list_simpl; apply IHpi2_1; list_simpl; reflexivity.
-  + rewrite <- app_assoc; apply tens_irr; [ assumption | ].
-    apply IHpi2_2; list_simpl; reflexivity.
+  + rewrite 2 app_assoc. apply tens_irr; [ | assumption ].
+    list_simpl. apply IHpi2_1. reflexivity.
+  + rewrite <- app_assoc. apply tens_irr; [ assumption | ].
+    apply IHpi2_2. reflexivity.
 - trichot_elt_elt_inf_exec Heql.
   + dichot_elt_app_inf_exec Heql1; subst.
-    * list_simpl; rewrite (app_assoc l), (app_assoc (l ++ l0)).
-      apply lpam_ilr; [ | assumption ].
-      list_simpl; apply IHpi2_1; reflexivity.
-    * list_simpl; apply lpam_ilr; [ assumption | ].
-      rewrite app_comm_cons, app_assoc; apply IHpi2_2; list_simpl; reflexivity.
-  + inversion Heql1.
-  + rewrite 2 app_assoc; apply lpam_ilr; [ assumption | ].
-    list_simpl; apply IHpi2_2; list_simpl; reflexivity.
+    * list_simpl. rewrite (app_assoc l), (app_assoc (l ++ l0)). apply lpam_ilr; [ | assumption ].
+      list_simpl. apply IHpi2_1. reflexivity.
+    * list_simpl. apply lpam_ilr; [ assumption | ].
+      rewrite app_comm_cons, app_assoc. apply IHpi2_2. list_simpl. reflexivity.
+  + discriminate Heql1.
+  + rewrite 2 app_assoc. apply lpam_ilr; [ assumption | ].
+    list_simpl. apply IHpi2_2. list_simpl. reflexivity.
 - destruct l1; inversion Heql; subst.
-  list_simpl; apply gen_ilr, IHpi2; reflexivity.
-- rewrite app_assoc in Heql; trichot_elt_elt_inf_exec Heql.
-  + list_simpl; apply lmap_ilr; [ assumption | ].
-    rewrite app_comm_cons, app_assoc; apply IHpi2_2; list_simpl; reflexivity.
-  + inversion Heql1.
+  list_simpl. apply gen_ilr, IHpi2. reflexivity.
+- rewrite app_assoc in Heql. trichot_elt_elt_inf_exec Heql.
+  + list_simpl. apply lmap_ilr; [ assumption | ].
+    rewrite app_comm_cons, app_assoc. apply IHpi2_2. list_simpl. reflexivity.
+  + discriminate Heql1.
   + dichot_elt_app_inf_exec Heql0; subst.
-    * list_simpl; rewrite 2 app_assoc.
-      apply lmap_ilr; [ assumption | ].
-      list_simpl; apply IHpi2_2; list_simpl; reflexivity.
-    * list_simpl; rewrite (app_assoc l6), (app_assoc (l6 ++ l0)).
-      apply lmap_ilr; [ | assumption ].
-      list_simpl; apply IHpi2_1; reflexivity.
+    * list_simpl. rewrite 2 app_assoc. apply lmap_ilr; [ assumption | ].
+      list_simpl. apply IHpi2_2. list_simpl. reflexivity.
+    * list_simpl. rewrite (app_assoc l6), (app_assoc (l6 ++ l0)). apply lmap_ilr; [ | assumption ].
+      list_simpl. apply IHpi2_1. reflexivity.
 - assert ({l2' | l2 = l2' ++ ineg A :: nil & l = l1 ++ ivar X :: l2' }) as [l2' -> ->].
-  { revert Heql; clear; induction l2 using rev_rect; intros Heq.
-    + exfalso.
-      assert (rev (l ++ ineg A :: nil) = rev (l1 ++ ivar X :: nil)) as Heqr by (f_equal; assumption).
-      rewrite 2 rev_unit in Heqr; inversion Heqr.
-    + rewrite app_comm_cons, app_assoc in Heq.
-      apply app_inj_tail in Heq as [-> ->].
+  { clear - Heql. induction l2 in Heql |- * using rev_rect.
+    + exfalso. enough (ineg A = ivar X) as Hd by discriminate Hd.
+      rewrite <- (last_last l1 (ivar X) (ivar X)), <- (last_last l (ineg A) (ivar X)), Heql. reflexivity.
+    + rewrite app_comm_cons, app_assoc in Heql. apply app_inj_tail in Heql as [-> ->].
       exists l2; reflexivity. }
-  rewrite 2 app_assoc; apply neg_ilr.
-  list_simpl; apply IHpi2; reflexivity.
+  rewrite 2 app_assoc. apply neg_ilr.
+  list_simpl. apply IHpi2. reflexivity.
 - apply with_irr; [ apply IHpi2_1 | apply IHpi2_2]; reflexivity.
 - trichot_elt_elt_inf_exec Heql.
-  + list_simpl; apply plus_ilr; rewrite app_comm_cons, app_assoc;
-      [ apply IHpi2_1 | apply IHpi2_2]; list_simpl; reflexivity.
-  + inversion Heql1.
-  + rewrite 2 app_assoc; apply plus_ilr; list_simpl;
-      [ apply IHpi2_1 | apply IHpi2_2]; list_simpl; reflexivity.
-- decomp_map_inf Heql; inversion Heql3.
+  + list_simpl.
+    apply plus_ilr; rewrite app_comm_cons, app_assoc; [ apply IHpi2_1 | apply IHpi2_2 ]; list_simpl; reflexivity.
+  + discriminate Heql1.
+  + rewrite 2 app_assoc.
+    apply plus_ilr; list_simpl; [ apply IHpi2_1 | apply IHpi2_2 ]; list_simpl; reflexivity.
+- decomp_map_inf Heql. discriminate.
 - trichot_elt_app_inf_exec Heql; subst.
-  + rewrite 2 app_assoc; apply cut_ir with A; try assumption.
-    list_simpl; apply IHpi2_2; list_simpl; reflexivity.
-  + destruct Heql1 as [<- ->].
-    list_simpl; rewrite (app_assoc l), (app_assoc (l ++ l0)).
-    apply cut_ir with A; try assumption.
-    list_simpl; apply IHpi2_1; list_simpl; reflexivity.
-  + list_simpl; apply cut_ir with A; try assumption.
-    rewrite app_comm_cons, app_assoc; apply IHpi2_2; list_simpl; reflexivity.
+  + rewrite 2 app_assoc. apply cut_ir with A; [ assumption .. | ].
+    list_simpl. apply IHpi2_2. list_simpl. reflexivity.
+  + list_simpl. rewrite (app_assoc l), (app_assoc (l ++ l0)). apply cut_ir with A; [ assumption | | assumption ].
+    list_simpl. apply IHpi2_1. reflexivity.
+  + list_simpl. apply cut_ir with A; [ assumption .. | ].
+    rewrite app_comm_cons, app_assoc. apply IHpi2_2. list_simpl. reflexivity.
 - apply subs_gax_l; assumption.
 Qed.
 
