yalla/ill_prop.v
@@ -18,23 +18,28 @@ Notation ill := (@ill preiatom).
 
 Lemma strong_consistency_ill_axfree P (Hgax : no_iax P) : notT (ill P nil izero).
 Proof.
-intros pi.
-apply cut_admissible_ill_axfree in pi; try assumption.
+intros pi%cut_admissible_ill_axfree; [ | assumption ].
 remember nil as l eqn:Heql. remember izero as C eqn:HeqC.
 induction pi in Heql, HeqC |- *; inversion Heql; inversion HeqC; subst;
   try now (destruct l1; inversion Heql).
-- apply IHpi; try reflexivity.
-  symmetry in p.
-  apply (PEPermutation_Type_nil _ _ p).
-- apply IHpi; try reflexivity.
-  destruct l1, lw', l2; inversion Heql.
-  symmetry in p. apply Permutation_Type_nil in p as ->. reflexivity.
-- destruct l1, l0; inversion Heql.
-- apply (Hgax a).
+- symmetry in p. apply PEPermutation_Type_nil in p as ->.
+  apply IHpi; reflexivity.
+- apply app_eq_nil in Heql as [-> [->%map_eq_nil ->]%app_eq_nil].
+  symmetry in p. apply Permutation_Type_nil in p as ->.
+  apply IHpi; reflexivity.
+- rewrite app_assoc in Heql. symmetry in Heql. nil_vs_elt_inv Heql.
+- contradiction (Hgax a).
 Qed.
 
 
 (** ** Relating negation and implication *)
+
+Lemma cut_N_ir P (Hgax : noN_iax P) l0 l1 l2 C :
+  ill P l0 N -> ill P (l1 ++ N :: l2) C -> ill P (l1 ++ l0 ++ l2) C.
+Proof.
+intros pi1 pi2. refine (cut_at_ir_gax Hgax _ _ _ pi1 pi2).
+intros b l l' Heq. exfalso. apply (Hgax b). rewrite Heq. apply in_inf_elt.
+Qed.
 
 Lemma ilmap_to_ineg P A : ill P (ilmap A N :: nil) (ineg A).
 Proof. apply neg_irr. cons2app. rewrite <- (app_nil_l _). apply lmap_ilr; apply ax_exp_ill. Qed.
@@ -44,12 +49,7 @@ Proof. apply lmap_irr. cons2app. apply neg_ilr, ax_exp_ill. Qed.
 
 Lemma neg_map_rule P (Hgax : noN_iax P) l0 l1 l2 C D :
   ill P l0 C -> ill P (l1 ++ N :: l2) D -> ill P (l1 ++ l0 ++ ineg C :: l2) D.
-Proof.
-intros pi0 pi. cons2app. rewrite (app_assoc l0).
-refine (cut_at_ir_gax Hgax _ _ _ (neg_ilr _ _ pi0) pi).
-intros b l l' Heq. exfalso.
-apply (Hgax b). rewrite Heq. apply in_inf_elt.
-Qed.
+Proof. intros pi0%neg_ilr pi. cons2app. rewrite (app_assoc l0). apply cut_N_ir; assumption. Qed.
 
 Lemma ilpam_to_igen P A : ill P (ilpam A N :: nil) (igen A).
 Proof.
@@ -62,93 +62,86 @@ Proof. apply lpam_irr, gen_ilr, ax_exp_ill. Qed.
 
 Lemma gen_pam_rule P (Hgax : noN_iax P) l0 l1 l2 C D :
   ill P l0 C -> ill P (l1 ++ N :: l2) D -> ill P (l1 ++ igen C :: l0 ++ l2) D.
-Proof.
-intros pi0 pi. rewrite app_comm_cons.
-refine (cut_at_ir_gax Hgax _ _ _ (gen_ilr _ _ pi0) pi).
-intros b l l' Heq. exfalso.
-apply (Hgax b). rewrite Heq. apply in_inf_elt.
-Qed.
+Proof. intros pi0%gen_ilr pi. rewrite app_comm_cons. apply cut_N_ir; assumption. Qed.
 
 
 (** ** Reversibility statements *)
 (** axiom-free cases *)
 
 Lemma ione_rev_noax P (Hgax : no_iax P) l1 l2 C : ill P (l1 ++ ione :: l2) C -> ill P (l1 ++ l2) C.
-Proof. intros pi. rewrite <- (app_nil_l l2). apply cut_ir_axfree with ione; (assumption + apply one_irr). Qed.
+Proof. intro pi. rewrite <- (app_nil_l l2). apply cut_ir_axfree with ione; (assumption + apply one_irr). Qed.
 
 Lemma itens_rev_noax P (Hgax : no_iax P) l1 l2 A B C :
   ill P (l1 ++ itens A B :: l2) C -> ill P (l1 ++ A :: B :: l2) C.
 Proof.
-intros pi.
+intro pi.
 assert (ill P (A :: B :: nil) (itens A B)) as Hax by (cons2app; apply tens_irr; apply ax_exp_ill).
 rewrite <- (app_nil_l l2), 2 app_comm_cons. eapply cut_ir_axfree; eassumption.
 Qed.
 
 Lemma ilpam_rev_noax P (Hgax : no_iax P) l A B : ill P l (ilpam A B) -> ill P (l ++ A :: nil) B.
 Proof.
-intros pi.
-assert (ill P (ilpam A B :: A :: nil) B) as Hax.
-{ rewrite <- (app_nil_r _), <- app_comm_cons, <- (app_nil_l _).
-  apply lpam_ilr; apply ax_exp_ill. }
+intro pi.
+assert (ill P (ilpam A B :: A :: nil) B) as Hax
+  by (rewrite <- (app_nil_r _), <- app_comm_cons, <- (app_nil_l _); apply lpam_ilr; apply ax_exp_ill).
 rewrite <- (app_nil_l _). eapply cut_ir_axfree; eassumption.
 Qed.
 
 Lemma igen_rev_noax P (Hgax : no_iax P) l A : ill P l (igen A) -> ill P (l ++ A :: nil) N.
 Proof.
-intros pi.
-assert (ill P (igen A :: A :: nil) N) as Hax by (apply gen_ilr; apply ax_exp_ill).
+intro pi.
+assert (ill P (igen A :: A :: nil) N) as Hax by apply gen_ilr, ax_exp_ill.
 rewrite <- (app_nil_l _). eapply cut_ir_axfree; eassumption.
 Qed.
 
 Lemma ilmap_rev_noax P (Hgax : no_iax P) l A B : ill P l (ilmap A B) -> ill P (A :: l) B.
 Proof.
-intros pi.
-assert (ill P (A :: ilmap A B :: nil) B) as Hax.
-{ cons2app. rewrite <- (app_nil_l (A :: _)), <- app_assoc.
-  apply lmap_ilr; apply ax_exp_ill. }
+intro pi.
+assert (ill P (A :: ilmap A B :: nil) B) as Hax
+  by (cons2app; rewrite <- (app_nil_l (A :: _)), <- app_assoc; apply lmap_ilr; apply ax_exp_ill).
 rewrite <- (app_nil_r _), <- (app_nil_l l), app_comm_cons, <- app_assoc. eapply cut_ir_axfree; eassumption.
 Qed.
 
 Lemma ineg_rev_noax P (Hgax : no_iax P) l A : ill P l (ineg A) -> ill P (A :: l) N.
 Proof.
-intros pi.
-assert (ill P (A :: ineg A :: nil) N) as Hax by (cons2app; apply neg_ilr; apply ax_exp_ill).
+intro pi.
+assert (ill P (A :: ineg A :: nil) N) as Hax by (cons2app; apply neg_ilr, ax_exp_ill).
 rewrite <- (app_nil_r _), <- (app_nil_l l), app_comm_cons, <- app_assoc. eapply cut_ir_axfree; eassumption.
 Qed.
 
 Lemma iwith_rev1_noax P (Hgax : no_iax P) l A B : ill P l (iwith A B) -> ill P l A.
 Proof.
-intros pi.
-assert (ill P (iwith A B :: nil) A) as Hax by (rewrite <- (app_nil_l _); apply with_ilr1; apply ax_exp_ill).
+intro pi.
+assert (ill P (iwith A B :: nil) A) as Hax by (rewrite <- (app_nil_l _); apply with_ilr1, ax_exp_ill).
 rewrite <- (app_nil_r _), <- (app_nil_l _). eapply cut_ir_axfree; eassumption.
 Qed.
 
 Lemma iwith_rev2_noax P (Hgax : no_iax P) l A B : ill P l (iwith B A) -> ill P l A.
 Proof.
-intros pi.
-assert (ill P (iwith B A :: nil) A) as Hax by (rewrite <- (app_nil_l _); apply with_ilr2; apply ax_exp_ill).
+intro pi.
+assert (ill P (iwith B A :: nil) A) as Hax by (rewrite <- (app_nil_l _); apply with_ilr2, ax_exp_ill).
 rewrite <- (app_nil_r _), <- (app_nil_l _). eapply cut_ir_axfree; eassumption.
 Qed.
 
 Lemma iplus_rev1_noax P (Hgax : no_iax P) l1 l2 A B C :
   ill P (l1 ++ iplus A B :: l2) C -> ill P (l1 ++ A :: l2) C.
 Proof.
-intros pi.
-assert (ill P (A :: nil) (iplus A B)) as Hax by (apply plus_irr1; apply ax_exp_ill).
+intro pi.
+assert (ill P (A :: nil) (iplus A B)) as Hax by apply plus_irr1, ax_exp_ill.
 rewrite <- (app_nil_l l2), app_comm_cons. eapply cut_ir_axfree; eassumption.
 Qed.
 
 Lemma iplus_rev2_noax P (Hgax : no_iax P) l1 l2 A B C :
   ill P (l1 ++ iplus B A :: l2) C -> ill P (l1 ++ A :: l2) C.
 Proof.
-intros pi.
-assert (ill P (A :: nil) (iplus B A)) as Hax by (apply plus_irr2; apply ax_exp_ill).
+intro pi.
+assert (ill P (A :: nil) (iplus B A)) as Hax by apply plus_irr2, ax_exp_ill.
 rewrite <- (app_nil_l l2), app_comm_cons. eapply cut_ir_axfree; eassumption.
 Qed.
 
 Lemma ioc_rev_noax P (Hgax : no_iax P) l A : ill P l (ioc A) -> ill P l A.
 Proof.
-intros pi.
+intro pi.
 assert (ill P (ioc A :: nil) A) as Hax by (rewrite <- (app_nil_l _); apply de_ilr, ax_exp_ill).
 rewrite <- (app_nil_r _), <- (app_nil_l _). eapply cut_ir_axfree; eassumption.
 Qed.
@@ -176,7 +169,7 @@ induction pi; cbn; intros HFS; inversion HFS as [|D l' Hhd Htl]; subst; repeat s
 - refine (Permutation_Type_Forall_inf _ Htl).
   symmetry in p. apply Permutation_Type_app_head, Permutation_Type_app_tail, Permutation_Type_map, p.
 - Forall_inf_cbn_hyp. subst. Forall_inf_solve_rec.
-  constructor; [ | constructor; [ | assumption ]].
+  constructor; [ | constructor; [ | assumption ] ].
   + eapply Hfrag; [ eassumption | now repeat constructor ].
   + eapply Hfrag; [ eassumption | now repeat constructor ].
 - rewrite P_cutfree in f. discriminate f.
@@ -190,47 +183,41 @@ Proof.
 apply (iconservativity P_cutfree).
 - intros C Hf B Hs.
   eapply Exists_impl, Hf.
-  intros D HCD.
-  transitivity C; assumption.
-- remember (A :: l) as l0. clear.
-  induction l0 as [|A l IHl]; constructor.
-  + constructor; constructor.
-  + eapply Forall_inf_arrow, IHl.
-    intros B Hl. right. exact Hl.
+  intros D HCD. transitivity C; assumption.
+- remember (A :: l) as l0. clear. induction l0 as [|A l IHl]; repeat constructor.
+  eapply Forall_inf_arrow, IHl.
+  intros B Hl. right. exact Hl.
 Qed.
 
 Lemma iconservativity_axfree P (P_axfree : no_iax P) FS (Hfrag : ifragment FS) l A (pi : ill P l A) :
   Forall_inf FS (A :: l) -> { pi' : ill P l A & Forall_iformula FS pi' }.
 Proof.
-intros HFS.
+intro HFS.
 apply cut_admissible_ill_axfree in pi; [ | assumption ].
 exists (stronger_ipfrag (cutrm_ipfrag_le P) pi).
-apply Forall_isequent_stronger_ipfrag, iconservativity; [ | assumption | assumption ].
+apply Forall_isequent_stronger_ipfrag, iconservativity; [ | assumption .. ].
 apply noicut_cutrm.
 Qed.
 
 Lemma cut_admissible_ifragment_axfree P (P_axfree : no_iax P) FS (Hfrag : ifragment FS) l A (pi : ill P l A) :
   Forall_iformula FS pi -> { pi' : ill (cutrm_ipfrag P) l A & Forall_iformula FS pi'}.
 Proof.
-intros HFS.
-apply iconservativity_axfree; [ assumption | assumption | | ].
+intro HFS.
+apply iconservativity_axfree; [ assumption .. | | ].
 - apply cut_admissible_ill_axfree; assumption.
-- apply (Forall_isequent_is _ _ HFS).
+- exact (Forall_isequent_is _ _ HFS).
 Qed.
 
-Lemma subformula P (P_axfree : no_iax P) l A (pi : ill P l A) :
+Lemma isubformula P (P_axfree : no_iax P) l A (pi : ill P l A) :
   { pi': ill P l A & Forall_iformula (fun x => Exists (isubform x) (A :: l)) pi' }.
 Proof.
 refine (iconservativity_axfree P_axfree _ pi _).
 - intros C Hf B Hs.
   eapply Exists_impl, Hf.
-  intros D HCD.
-  transitivity C; assumption.
-- remember (A :: l) as l0. clear.
-  induction l0 as [|A l IHl]; constructor.
-  + constructor; constructor.
-  + eapply Forall_inf_arrow, IHl.
-    intros B Hl. right. exact Hl.
+  intros D HCD. transitivity C; assumption.
+- remember (A :: l) as l0. clear. induction l0 as [|A l IHl]; repeat constructor.
+  eapply Forall_inf_arrow, IHl.
+  intros B Hl. right. exact Hl.
 Qed.
 
 End Atoms.
