yalla/ll_cut_at.v
@@ -12,8 +12,7 @@ Lemma cut_gax_l At P A a l1 l2 l3 l4 :
   (forall b l l', projT2 (pgax P) b = (l ++ A :: l') -> ll P (l1 ++ l' ++ l ++ l2)) ->
   ll P (l3 ++ A :: l4) -> @ll At P (l1 ++ l4 ++ l3 ++ l2).
 Proof.
-intros Hat Hgax Hcut pi.
-remember (l3 ++ A :: l4) as l.
+intros Hat Hgax Hcut pi. remember (l3 ++ A :: l4) as l eqn:Heql.
 revert l3 l4 Heql. induction pi using ll_nested_ind; intros l4 l5 Heq; subst.
 - destruct l4; inversion Heq; subst.
   + cbn in Hgax. list_simpl. rewrite <- Hgax; apply (gax_r a).
@@ -33,7 +32,7 @@ revert l3 l4 Heql. induction pi using ll_nested_ind; intros l4 l5 Heq; subst.
      apply (ex_wn_r _ lw); [ list_simpl | assumption ].
      rewrite (app_assoc l), (app_assoc _ l3), <- (app_assoc l).
      now apply IHpi; list_simpl.
-  + destruct Heq1 as [Heq1 Heq2]; symmetry in Heq1; decomp_map_inf Heq1.
+  + symmetry in Heq1. decomp_map_inf Heq1.
     exfalso. rewrite <- Heq1 in Hat. inversion Hat.
   + list_simpl. rewrite 2 app_assoc.
     apply (ex_wn_r _ lw); [ | assumption ].
@@ -56,9 +55,7 @@ revert l3 l4 Heql. induction pi using ll_nested_ind; intros l4 l5 Heq; subst.
       [ | list_simpl; rewrite app_assoc, (app_assoc _ l2); apply PCPermutation_Type_app_comm ].
     destruct (In_Forall_inf_elt _ _ (l1' ++ A :: l2') PL) as [pi Hin].
     refine (Dependent_Forall_inf_forall_formula _ _ X Hin _ _ eq_refl).
-- exfalso. destruct l4; inversion Heq.
-  + rewrite <- H0 in Hat. inversion Hat.
-  + destruct l4; inversion H1.
+- exfalso. unit_vs_elt_inv Heq. inversion Hat.
 - destruct l4; inversion Heq; subst; try (exfalso; inversion Hat; fail).
   eapply ex_r; [ | apply PCPermutation_Type_app_rot ]; list_simpl.
   apply bot_r.
@@ -144,20 +141,16 @@ Proof.
 enough (forall s A l0 l1 l2 (pi1: ll P (A :: l0)) (pi2 : ll P (l1 ++ dual A :: l2)),
        s = psize pi1 + psize pi2 -> { A = var X } + { A = covar X } -> ll P (l1 ++ l0 ++ l2))
   as Hat.
-{ intros pi1 pi2.
-  eapply ex_r; [ | apply PCPermutation_Type_app_comm ].
-  rewrite app_assoc, <- 2 app_assoc.
-  eapply ex_r; [ | apply PCPermutation_Type_app_comm ].
-  rewrite <- app_assoc.
-  apply (ex_r _ ((var X :: l2) ++ l1)) in pi1; [ | apply PCPermutation_Type_app_comm ].
+{ intros pi1 pi2. eapply ex_r; [ | apply PCPermutation_Type_app_comm ].
+  rewrite app_assoc, <- 2 app_assoc. eapply ex_r; [ | apply PCPermutation_Type_app_comm ].
+  rewrite <- app_assoc. apply (ex_r _ ((var X :: l2) ++ l1)) in pi1; [ | apply PCPermutation_Type_app_comm ].
   rewrite <- app_comm_cons in pi1.
-  refine (Hat (psize pi1 + psize pi2) (var X) (l2 ++ l1) l3 l4 pi1 pi2 _ _); [ reflexivity | ].
-  left. reflexivity. }
+  refine (Hat (psize pi1 + psize pi2) (var X) (l2 ++ l1) l3 l4 pi1 pi2 _ _); [ | left ]; reflexivity. }
 clear l1 l2 l3 l4.
 induction s as [s IHsize0] using lt_wf_rect; intros A l0 l1 l2 pi1 pi2 -> Hat.
-remember (l1 ++ dual A :: l2) as l; destruct_ll pi2 f Y l Hl Hr HP FL a; cbn in IHsize0.
+remember (l1 ++ dual A :: l2) as l eqn:Heql. destruct_ll pi2 f Y l Hl Hr HP FL a; cbn in IHsize0.
 - destruct l1; inversion Heql; subst.
-  + apply codual in H0; cbn; subst.
+  + apply codual in H0. cbn. subst.
     eapply ex_r; [ | apply PCPermutation_Type_app_comm ]; assumption.
   + destruct l1; inversion H1; [ | destruct l1; inversion H2 ]; subst.
     apply codual in H0; cbn; subst; list_simpl; assumption.
@@ -166,119 +159,103 @@ remember (l1 ++ dual A :: l2) as l; destruct_ll pi2 f Y l Hl Hr HP FL a; cbn in 
   refine (ex_r _ _ _ HP).
   refine (IHsize0 (psize pi1 + psize Hl) _ _ _ _ _ pi1 Hl _ Hat); lia.
 - trichot_elt_app_inf_exec Heql; subst.
-  + rewrite 2 app_assoc.
-    eapply ex_wn_r; [ | apply HP ].
-    revert Hl IHsize0; list_simpl; intros Hl IHsize0.
+  + rewrite 2 app_assoc. eapply ex_wn_r; [ | apply HP ].
+    revert Hl IHsize0. list_simpl. intros Hl IHsize0.
     refine (IHsize0 (psize pi1 + psize Hl) _ _ _ _ _ pi1 Hl _ Hat); lia.
-  + destruct Heql1 as [H _].
-    symmetry in H; decomp_map_inf H.
-    destruct Hat as [-> | ->]; inversion H3.
-  + list_simpl.
-    eapply ex_wn_r; [ | apply HP ].
-    revert Hl IHsize0; rewrite 2 app_assoc; intros Hl IHsize0.
-    rewrite 2 app_assoc.
+  + symmetry in Heql1. decomp_map_inf Heql1.
+    destruct Hat as [-> | ->]; discriminate Heql1.
+  + list_simpl. eapply ex_wn_r; [ | apply HP ].
+    revert Hl IHsize0. rewrite 2 app_assoc. intros Hl IHsize0. rewrite 2 app_assoc.
     refine (IHsize0 (psize pi1 + psize Hl) _ _ _ _ _ pi1 Hl _ Hat); lia.
 - apply concat_vs_elt in Heql as ((((L1 &L2) & l1') & l2') & (Heqb & (Heqt & HeqL))); subst.
   rewrite <- app_assoc.
   replace (l1' ++ l0 ++ l2' ++ concat L2)
      with ((l1' ++ l0 ++ l2') ++ concat L2) by (rewrite ? app_assoc; reflexivity).
   change ((l1' ++ l0 ++ l2') ++ concat L2) with (concat ((l1' ++ l0 ++ l2') :: L2)).
-  rewrite <- concat_app.
-  apply mix_r.
-  + rewrite app_length.
-    rewrite app_length in f; cbn; cbn in f; assumption.
+  rewrite <- concat_app. apply mix_r.
+  + rewrite app_length. rewrite app_length in f. cbn. cbn in f. assumption.
   + assert (FL1 := Forall_inf_app_l _ _ FL).
     assert (FL2 := Forall_inf_app_r _ _ FL).
-    inversion FL2; subst; clear FL2; rename X1 into FL2; rename X0 into pi.
+    inversion FL2. subst. clear FL2. rename X1 into FL2. rename X0 into pi.
     apply Forall_inf_app; [ assumption | ].
     apply Forall_inf_cons; [ | assumption ].
     clear pi.
     destruct (In_Forall_inf_elt _ _ (l1' ++ dual A :: l2') FL) as [pi Hin].
     refine (IHsize0 _ _ _ _ _ _ pi1 pi _ _); [ | reflexivity | assumption ].
     assert (psize pi < psize (mix_r f FL)) as H by (eapply psize_inf_mix; eassumption).
-    cbn in H; lia.
-- destruct l1; inversion Heql; [ | destruct l1; inversion H1 ].
-  destruct Hat as [-> | ->]; inversion H0.
+    cbn in H. lia.
+- unit_vs_elt_inv Heql. destruct Hat as [-> | ->]; discriminate Heql.
 - destruct l1; inversion Heql; subst.
-  + destruct Hat as [-> | ->]; inversion H0.
-  + cbn; apply bot_r.
+  + destruct Hat as [-> | ->]; discriminate H0.
+  + cbn. apply bot_r.
     refine (IHsize0 (psize pi1 + psize Hl) _ _ _ _ _ pi1 Hl _ Hat); lia.
 - destruct l1; inversion Heql; subst.
-  + destruct Hat as [-> | ->]; inversion H0.
+  + destruct Hat as [-> | ->]; discriminate H0.
   + dichot_elt_app_inf_exec H1; subst.
-    * list_simpl; rewrite 2 app_assoc; apply tens_r; [ assumption | ].
-      list_simpl; rewrite app_comm_cons.
-      revert Hr IHsize0; rewrite app_comm_cons; intros Hr IHsize0.
+    * list_simpl. rewrite 2 app_assoc. apply tens_r; [ assumption | ].
+      list_simpl. rewrite app_comm_cons. revert Hr IHsize0. rewrite app_comm_cons. intros Hr IHsize0.
       refine (IHsize0 (psize pi1 + psize Hr) _ _ _ _ _ pi1 Hr _ Hat); lia.
-    * list_simpl; apply tens_r; [ | assumption ].
-      list_simpl; rewrite app_comm_cons.
-      revert Hl IHsize0; rewrite app_comm_cons; intros Hl IHsize0.
+    * list_simpl. apply tens_r; [ | assumption ].
+      list_simpl. rewrite app_comm_cons. revert Hl IHsize0. rewrite app_comm_cons. intros Hl IHsize0.
       refine (IHsize0 (psize pi1 + psize Hl) _ _ _ _ _ pi1 Hl _ Hat); lia.
 - destruct l1; inversion Heql; subst.
-  + destruct Hat as [-> | ->]; inversion H0.
-  + cbn; apply parr_r.
-    revert Hl IHsize0; rewrite 2 app_comm_cons; intros Hl IHsize0.
+  + destruct Hat as [-> | ->]; discriminate H0.
+  + cbn. apply parr_r.
+    revert Hl IHsize0. rewrite 2 app_comm_cons. intros Hl IHsize0.
     refine (IHsize0 (psize pi1 + psize Hl) _ _ _ _ _ pi1 Hl _ Hat); lia.
 - destruct l1; inversion Heql; subst.
-  + destruct Hat as [-> | ->]; inversion H0.
+  + destruct Hat as [-> | ->]; discriminate H0.
   + apply top_r.
 - destruct l1; inversion Heql; subst.
-  + destruct Hat as [-> | ->]; inversion H0.
+  + destruct Hat as [-> | ->]; discriminate H0.
   + cbn; apply plus_r1.
-    revert Hl IHsize0; rewrite app_comm_cons; intros Hl IHsize0.
+    revert Hl IHsize0. rewrite app_comm_cons. intros Hl IHsize0.
     refine (IHsize0 (psize pi1 + psize Hl) _ _ _ _ _ pi1 Hl _ Hat); lia.
 - destruct l1; inversion Heql; subst.
-  + destruct Hat as [-> | ->]; inversion H0.
-  + cbn; apply plus_r2.
-    revert Hl IHsize0; rewrite app_comm_cons; intros Hl IHsize0.
+  + destruct Hat as [-> | ->]; discriminate H0.
+  + cbn. apply plus_r2.
+    revert Hl IHsize0. rewrite app_comm_cons. intros Hl IHsize0.
     refine (IHsize0 (psize pi1 + psize Hl) _ _ _ _ _ pi1 Hl _ Hat); lia.
 - destruct l1; inversion Heql; subst.
-  + destruct Hat as [-> | ->]; inversion H0.
-  + cbn; apply with_r.
-    * revert Hl IHsize0; rewrite app_comm_cons; intros Hl IHsize0.
+  + destruct Hat as [-> | ->]; discriminate H0.
+  + cbn. apply with_r.
+    * revert Hl IHsize0. rewrite app_comm_cons. intros Hl IHsize0.
       refine (IHsize0 (psize pi1 + psize Hl) _ _ _ _ _ pi1 Hl _ Hat); lia.
-    * revert Hr IHsize0; rewrite app_comm_cons; intros Hr IHsize0.
+    * revert Hr IHsize0. rewrite app_comm_cons. intros Hr IHsize0.
       refine (IHsize0 (psize pi1 + psize Hr) _ _ _ _ _ pi1 Hr _ Hat); lia.
 - destruct l1; inversion Heql; subst.
-  + destruct Hat as [-> | ->]; inversion H0.
+  + destruct Hat as [-> | ->]; discriminate H0.
   + decomp_map_inf H1.
-    destruct Hat as [-> | ->]; inversion H1.
+    destruct Hat as [-> | ->]; discriminate H1.
 - destruct l1; inversion Heql; subst.
-  + destruct Hat as [-> | ->]; inversion H0.
-  + cbn; apply de_r.
-    revert Hl IHsize0; rewrite app_comm_cons; intros Hl IHsize0.
+  + destruct Hat as [-> | ->]; discriminate H0.
+  + cbn. apply de_r.
+    revert Hl IHsize0. rewrite app_comm_cons. intros Hl IHsize0.
     refine (IHsize0 (psize pi1 + psize Hl) _ _ _ _ _ pi1 Hl _ Hat); lia.
 - destruct l1; inversion Heql; subst.
-  + destruct Hat as [-> | ->]; inversion H0.
-  + cbn; apply wk_r.
+  + destruct Hat as [-> | ->]; discriminate H0.
+  + cbn. apply wk_r.
     refine (IHsize0 (psize pi1 + psize Hl) _ _ _ _ _ pi1 Hl _ Hat); lia.
 - destruct l1; inversion Heql; subst.
-  + destruct Hat as [-> | ->]; inversion H0.
-  + cbn; apply co_r.
-    revert Hl IHsize0; rewrite 2 app_comm_cons; intros Hl IHsize0.
+  + destruct Hat as [-> | ->]; discriminate H0.
+  + cbn. apply co_r.
+    revert Hl IHsize0. rewrite 2 app_comm_cons. intros Hl IHsize0.
     refine (IHsize0 (psize pi1 + psize Hl) _ _ _ _ _ pi1 Hl _ Hat); lia.
 - dichot_elt_app_inf_exec Heql; subst.
-  + rewrite 2 app_assoc.
-    apply (cut_r _ f); [ assumption | ].
-    list_simpl; rewrite app_comm_cons.
-    revert Hr IHsize0; rewrite app_comm_cons; intros Hr IHsize0.
+  + rewrite 2 app_assoc. apply (cut_r _ f); [ assumption | ].
+    list_simpl. rewrite app_comm_cons. revert Hr IHsize0. rewrite app_comm_cons. intros Hr IHsize0.
     refine (IHsize0 (psize pi1 + psize Hr) _ _ _ _ _ pi1 Hr _ Hat); lia.
-  + list_simpl.
-    apply (cut_r _ f); [ | assumption ].
-    list_simpl; rewrite app_comm_cons.
-    revert Hl IHsize0; rewrite app_comm_cons; intros Hl IHsize0.
+  + list_simpl. apply (cut_r _ f); [ | assumption ].
+    list_simpl. rewrite app_comm_cons. revert Hl IHsize0. rewrite app_comm_cons. intros Hl IHsize0.
     refine (IHsize0 (psize pi1 + psize Hl) _ _ _ _ _ pi1 Hl _ Hat); lia.
 - destruct Hat as [-> | ->].
   + rewrite <- (app_nil_r l0), <- app_assoc.
-    apply cut_gax_l with (var X) a; try assumption.
-    * constructor.
-    * intros b l l' Hb.
-      destruct (P_gax_cut b a _ _ _ _ Hb Heql) as [c <-]. apply gax_r.
+    apply cut_gax_l with (var X) a; [ constructor | assumption | | assumption ].
+    intros b l l' Hb. destruct (P_gax_cut b a _ _ _ _ Hb Heql) as [c <-]. apply gax_r.
   + rewrite <- (app_nil_r l0), <- app_assoc.
-    apply cut_gax_l with (covar X) a; try assumption.
-    * constructor.
-    * intros b l l' Hb.
-      apply (ex_r (l ++ l2 ++ l1 ++ l'));
-        [ | rewrite app_assoc, (app_assoc l1); apply PCPermutation_Type_app_comm ].
-      destruct (P_gax_cut a b _ _ _ _ Heql Hb) as [c <-]. apply gax_r.
+    apply cut_gax_l with (covar X) a; [ constructor | assumption | | assumption ].
+    intros b l l' Hb.
+    apply (ex_r (l ++ l2 ++ l1 ++ l'));
+      [ | rewrite app_assoc, (app_assoc l1); apply PCPermutation_Type_app_comm ].
+    destruct (P_gax_cut a b _ _ _ _ Heql Hb) as [c <-]. apply gax_r.
 Qed.
