yalla/mell2.v
@@ -57,7 +57,7 @@ Lemma mell2ll_dual A : formulas.dual (mell2ll A) = mell2ll (dual A).
 Proof. induction A; cbn; rewrite ? IHA, ? IHA1, ? IHA2; reflexivity. Qed.
 
 Lemma mell2ll_map_wn l : map mell2ll (map wn l) = map formulas.wn (map mell2ll l).
-Proof. induction l as [ | A l IHl ]; [ reflexivity | cbn; f_equal; apply IHl ]. Qed.
+Proof. induction l as [ | A l IHl ]; [ | cbn; rewrite IHl ]; reflexivity. Qed.
 
 Lemma mell2ll_map_wn_inv l1 l2 : map formulas.wn l1 = map mell2ll l2 ->
   { l2' | l2 = map wn l2' & l1 = map mell2ll l2' }.
@@ -98,75 +98,66 @@ Definition pfrag_mell := @ll_def.mk_pfrag atom  ll_def.pcut_none ll_def.NoAxioms
 
 Lemma mell2mellfrag l : mell l -> ll_def.ll pfrag_mell (map mell2ll l).
 Proof.
-intros pi; induction pi; try (now constructor); rewrite ? map_app.
+intro pi. induction pi; try (constructor; assumption); rewrite ? map_app.
 - eapply ll_def.ex_r; [ apply IHpi | ].
-  apply Permutation_Type_map; assumption.
+  apply Permutation_Type_map. assumption.
 - replace (map mell2ll l1 ++ map mell2ll l2)
      with (concat (map mell2ll l1 :: map mell2ll l2 :: nil))
     by (cbn; rewrite app_nil_r; reflexivity).
-  apply ll_def.mix_r; now repeat constructor.
+  apply ll_def.mix_r; repeat constructor; assumption.
 - eapply ll_def.ex_r.
-  + apply (ll_def.tens_r IHpi1 IHpi2).
-  + cbn; rewrite map_app; apply Permutation_Type_cons, Permutation_Type_app_comm; reflexivity.
-- cbn; rewrite mell2ll_map_wn.
-  apply ll_def.oc_r.
-  rewrite <- mell2ll_map_wn; assumption.
+  + exact (ll_def.tens_r IHpi1 IHpi2).
+  + cbn. rewrite map_app. apply Permutation_Type_cons, Permutation_Type_app_comm. reflexivity.
+- cbn. rewrite mell2ll_map_wn. apply ll_def.oc_r.
+  rewrite <- mell2ll_map_wn. assumption.
 Qed.
 
 Lemma mellfrag2mell l : ll_def.ll pfrag_mell (map mell2ll l) -> mell l.
 Proof.
-intros pi.
-remember (map mell2ll l) as l0 eqn:Heql0.
-revert l Heql0; induction pi using ll_def.ll_nested_ind; intros l' Heql0; subst;
+intro pi. remember (map mell2ll l) as l0 eqn:Heql0.
+revert l Heql0. induction pi using ll_def.ll_nested_ind; intros l' Heql0; subst;
   try now (destruct l'; inversion Heql0; destruct f; inversion H0).
-- symmetry in Heql0; decomp_map_inf Heql0; subst.
+- symmetry in Heql0. decomp_map_inf Heql0. subst.
   destruct l1; inversion Heql4.
   destruct x; inversion Heql2; subst.
   destruct x0; inversion Heql0; subst.
   apply ax_r.
-- cbn in p.
-  apply Permutation_Type_map_inv in p as [l'' Heq HP%Permutation_Type_sym].
+- cbn in p. apply Permutation_Type_map_inv in p as [l'' Heq HP%Permutation_Type_sym].
   eapply ex_r, HP.
-  apply (IHpi _ Heq).
-- symmetry in Heql0; decomp_map_inf Heql0; subst; symmetry in Heql0.
-  cbn in Heql0; apply mell2ll_map_wn_inv in Heql0 as [l -> ->].
+  exact (IHpi _ Heq).
+- symmetry in Heql0. decomp_map_inf Heql0. subst. symmetry in Heql0.
+  apply mell2ll_map_wn_inv in Heql0 as [l -> ->].
   apply Permutation_Type_map_inv in p as [l' -> HP%Permutation_Type_sym].
-  eapply ex_r; [ apply IHpi; rewrite <- mell2ll_map_wn, <- ? map_app; reflexivity | ].
+  eapply ex_r; [ apply IHpi; rewrite <- mell2ll_map_wn, <- ! map_app; reflexivity | ].
   apply Permutation_Type_app_head, Permutation_Type_app_tail, Permutation_Type_map, HP.
 - remember (length L) as n eqn:Heqn.
   repeat (destruct n; inversion eqpmix).
   repeat (destruct L; inversion Heqn).
-  cbn in Heql0; symmetry in Heql0; decomp_map_inf Heql0; subst.
-  cbn in *; clear H0 H1 H2 H3 Heqn eqpmix.
-  destruct l5; inversion Heql4; rewrite app_nil_r; clear Heql4.
+  cbn in Heql0. symmetry in Heql0. decomp_map_inf Heql0. subst.
+  apply map_eq_nil in Heql4 as ->. rewrite app_nil_r.
   apply mix_r.
   + destruct (In_Forall_inf_in (map mell2ll l2) PL); [ left; reflexivity | ].
-    apply (ll_def.Dependent_Forall_inf_forall_formula _ _ X i _ eq_refl).
+    exact (ll_def.Dependent_Forall_inf_forall_formula _ _ X i _ eq_refl).
   + destruct (In_Forall_inf_in (map mell2ll l4) PL); [ right; left; reflexivity | ].
-    apply (ll_def.Dependent_Forall_inf_forall_formula _ _ X i _ eq_refl).
-- symmetry in Heql0; decomp_map_inf Heql0; subst.
-  destruct x; inversion Heql2; subst.
+    exact (ll_def.Dependent_Forall_inf_forall_formula _ _ X i _ eq_refl).
+- symmetry in Heql0. decomp_map_inf Heql0. subst.
+  destruct x; inversion Heql2. subst.
   eapply ex_r; [ apply tens_r | ].
-  + apply IHpi1; reflexivity.
-  + apply IHpi2; reflexivity.
-  + apply Permutation_Type_cons, Permutation_Type_app_comm; reflexivity.
-- destruct l'; inversion Heql0.
-  destruct f; inversion H0; subst.
-  apply parr_r, IHpi; reflexivity.
-- destruct l'; inversion Heql0.
-  destruct f; inversion H0; subst.
-  apply mell2ll_map_wn_inv in H1 as [l'' -> ->].
+  + apply IHpi1. reflexivity.
+  + apply IHpi2. reflexivity.
+  + apply Permutation_Type_cons, Permutation_Type_app_comm. reflexivity.
+- destruct l' as [|f l']; inversion Heql0 as [[Hf Heq]]. destruct f; inversion Hf. subst.
+  apply parr_r, IHpi. reflexivity.
+- destruct l' as [|f l']; inversion Heql0 as [[Hf Heq]]. destruct f; inversion Hf. subst.
+  apply mell2ll_map_wn_inv in Heq as [l'' -> ->].
   apply oc_r, IHpi.
-  cbn; rewrite mell2ll_map_wn; reflexivity.
-- destruct l'; inversion Heql0.
-  destruct f; inversion H0; subst.
-  apply de_r, IHpi; reflexivity.
-- destruct l'; inversion Heql0.
-  destruct f; inversion H0; subst.
-  apply wk_r, IHpi; reflexivity.
-- destruct l'; inversion Heql0.
-  destruct f; inversion H0; subst.
-  apply co_r, IHpi; reflexivity.
+  cbn. rewrite mell2ll_map_wn. reflexivity.
+- destruct l' as [|f l']; inversion Heql0 as [[Hf Heq]]. destruct f; inversion Hf. subst.
+  apply de_r, IHpi. reflexivity.
+- destruct l' as [|f l']; inversion Heql0 as [[Hf Heq]]. destruct f; inversion Hf. subst.
+  apply wk_r, IHpi. reflexivity.
+- destruct l' as [|f l']; inversion Heql0 as [[Hf Heq]]. destruct f; inversion Hf. subst.
+  apply co_r, IHpi. reflexivity.
 - discriminate f.
 - destruct a.
 Qed.
